\documentclass{article}

\author{Aidan Ewart}
\title{Formalization of ATT}

\usepackage{amsmath}
\usepackage{amsfonts}
\usepackage{syntax}
\usepackage{mathpartir}

\newcommand{\set}{\mathcal{U}}
\newcommand{\W}{\mathcal{W}}
\newcommand{\V}{\mathcal{V}}
\newcommand{\nat}{\mathbb{N}}
\newcommand{\fin}{\mathbb{F}}
\newcommand{\prop}{\mathbb{P}}
\newcommand{\elim}{\mathrm{elim}}
\newcommand{\rec}{\mathrm{rec}}
\newcommand{\tx}[1]{\mathrm{#1}}

\newcommand{\fun}[2]{\lambda #1. #2}
\newcommand{\for}[2]{\Pi_{#1}#2}

\newcommand{\bnfdef}{\hspace{0.5cm} ::= \hspace{0.5cm}}
\newcommand{\alt}{\hspace{0.25cm} | \hspace{0.25cm}}

\newcommand{\bb}{\mathbf}
\newcommand{\evals}{\rightsquigarrow^{nf}}

\begin{document}
\begin{align*}
    \bb{M} \bnfdef&
        x
        \tag{Type Variables}
    \\\alt&
        c
        \tag{Constant Types}
    \\\alt&
        \bb{M} \to \bb{M}
        \tag{Functions}
    \\\alt&
        \prop
        \tag{Propositions}
    \\\\\bb{S} \bnfdef&
        \forall{\bar{x}}, \bb{M}
        \tag{Type Schemes}
    \\\\\bb{T} \bnfdef&
        x
        \tag{Constants \& Variables}
    \\\alt&
        M
        \tag{Metavariables}
    \\\alt&
        \lambda x, \bb{T}
        \tag{$\lambda$-Abstractions}
    \\\alt&
        \bb{T} \bb{T}
        \tag{Application}
    \\\alt&
        \text{let $x$ = $\bb{T}$ in $\bb{T}$}
        \tag{Let-In}
    \\\alt&
        \Pi_{x : \bb{M}} \bb{T}
        \tag{$\forall$-Quantifiers}
    \\\alt&
        \bb{T} \Rightarrow \bb{T}
        \tag{Implication}
    \\\\\bb{P} \bnfdef&
        x
        \tag{Axioms \& Variables}
    \\\alt&
        \_
        \tag{Holes}
    \\\alt&
        \lambda_{\mathrm{Thm}} (x : \bb{T}), \bb{P}
        \tag{Implication Introduction}
    \\\alt&
        \bb{P} \$ \bb{P}
        \tag{Modus Ponens}
    \\\alt&
        \lambda_{\mathrm{Obj}} (x : \bb{S}), \bb{P}
        \tag{Universal Introduction}
    \\\alt&
        \bb{P}[x := \bb{T}]
        \tag{Universal Elimination}
\end{align*}

\begin{mathpar}
    \and \infer[Var]
        {(x, \tau) \in \Gamma}
        {\Gamma \vdash x : \tau}
    \and \infer[MetaVar]
        {(M, \tau) \in \Gamma}
        {\Gamma \vdash M : \tau}
    \and \infer[Lam]
        {\Gamma, (x, \tau_0) \vdash e : \tau_1}
        {\Gamma \vdash \lambda x. e : \tau_0 \to \tau_1}
    \and \infer[Forall]
        {\Gamma, (x, \tau) \vdash e : \prop}
        {\Gamma \vdash \Pi_{x : \tau} e : \prop}
    \and \infer[App]
        {\Gamma \vdash e_0 : \tau_0 \to \tau_1
        \\\Gamma \vdash e_1 : \tau_0}
        {\Gamma \vdash e_0 e_1 : \tau_1}
    \and \infer[Imp]
        {\Gamma \vdash e_0 : \prop
        \\\Gamma \vdash e_1 : \prop}
        {\Gamma \vdash e_0 \Rightarrow e_1 : \prop}
    \and \infer[Let]
        {\Gamma \vdash e_0 : \tau_0
        \\\bar{a} = \{a \in \text{free} (\tau_0) : a \notin \text{free} (\Gamma)\}
        \\\Gamma,(x, \forall \bar{a}. \tau_0) \vdash e_1 : \tau_1}
        {\Gamma \vdash \text{let $x$ = $e_0$ in $e_1$} : e_1}
\end{mathpar}

\begin{mathpar}
    \infer[Param]
        {(x, e) \in \Gamma}
        {\Gamma \vdash x : e}
    \and \infer[IntroThm]
        {\Gamma \vdash e_0 : \mathbb{P}
        \\\Gamma, (x, e_0) \vdash p : e_1}
        {\Gamma \vdash \lambda_{\mathrm{Thm}} (x : e_0), p : e_0 \Rightarrow e_1}
    \and \infer[ModPon]
        {\Gamma \vdash p_0 : e_0 \Rightarrow e_1
        \\\Gamma \vdash p_1 : e_0}
        {\Gamma \vdash p_0 \$ p_1 : e_1}
    \and \infer[IntroObj]
        {\Gamma, (x : \tau) \vdash p : e}
        {\Gamma \vdash \lambda_{\mathrm{Obj}} (x : \tau), p : \Pi_{x : \tau}, e}
    \and \infer[UniElim]
        {\Gamma \vdash e_0 : \tau
        \\\Gamma \vdash p : \Pi_{x : \tau} e_1}
        {\Gamma \vdash p[x := e_0] : e_1}
    \and \infer[Hole]
        { }
        {\Gamma \vdash \_ : e}
\end{mathpar}

\begin{mathpar}
    \infer[$\beta$-reduction]
        {\Gamma \vdash e_0 \rightsquigarrow (\lambda x. e_2)
        \\\Gamma \vdash e_2[x := e_1] \rightsquigarrow e_3}
        {\Gamma \vdash e_0 e_1 \rightsquigarrow e_3}
    \and \infer[Let-reduction]
        {\Gamma \vdash e_1[x := e_0] \rightsquigarrow e_2}
        {\Gamma \vdash \text{let $x$ = $e_0$ in $e_1$} \rightsquigarrow e_2}
    \and \infer[BindL]
        {M \notin x
        \\\text{subst}(M,y) \in \Gamma
        \\\Gamma \vdash y \sim x}
        {\Gamma \vdash M \sim x}
    \and \infer[BindR]
        {M \notin x
        \\\text{subst}(M,y) \in \Gamma
        \\\Gamma \vdash x \sim y}
        {\Gamma \vdash x \sim M}
    \and \infer[UnifyLambda]
        {\Gamma \vdash e_0 \sim e_1}
        {\Gamma \vdash (\lambda x. e_0) \sim (\lambda x. e_1)}
    \and \infer[UnifyForall]
        {\Gamma \vdash e_0 \sim e_1}
        {\Gamma \vdash (\Pi_{x : \tau}, e_0) \sim (\Pi_{x : \tau}, e_1)}
    \and \infer[UnifyApp]
        {\Gamma \vdash e_0 \sim e_2
        \\\Gamma \vdash e_1 \sim e_3}
        {\Gamma \vdash e_0 e_1 \sim e_2 e_3}
    \and \infer[UnifyImp]
        {\Gamma \vdash e_0 \sim e_2
        \\\Gamma \vdash e_1 \sim e_3}
        {\Gamma \vdash e_0 \Rightarrow e_1 \sim e_2 \Rightarrow e_3}
    \and \infer[ReduceL]
        {\Gamma \vdash e_0 \rightsquigarrow e_2
        \\\Gamma \vdash e_2 \sim e_1}
        {\Gamma \vdash e_0 \sim e_1}
    \and \infer[ReduceR]
        {\Gamma \vdash e_1 \rightsquigarrow e_2
        \\\Gamma \vdash e_0 \sim e_2}
        {\Gamma \vdash e_0 \sim e_1}
    \and \infer[Refl]
        { }
        {\Gamma \vdash e \sim e}
\end{mathpar}

\begin{mathpar}

\end{mathpar}

\end{document}